src/DirName.v
@@ -214,20 +214,19 @@ Module SDIR.
     let2 (mscs, r) <- DIR.dlink lxp bxp ixp dnum (string2name 16 name) inum mscs;
     rx (mscs, r).
 
-  Definition dslist T lxp ixp dnum mscs rx : prog T :=
-    let2 (mscs, r) <- DIR.dlist lxp ixp dnum mscs;
+  Definition dslist T lxp bxp ixp dnum mscs rx : prog T :=
+    let2 (mscs, r) <- DIR.dlist lxp bxp ixp dnum mscs;
     rx (mscs, List.map (fun di => (name2string 16 (fst di), snd di)) r).
 
-  Definition rep f (dsmap : @mem string string_dec addr) := (exists dmap, DIR.rep f dmap *
+  Definition rep F1 F2 m bxp ixp inum (dsmap : @mem string string_dec addr) :=
+   (exists dmap, DIR.rep F1 F2 m bxp ixp inum dmap *
     [[ True ]])%pred.
   (* XXX should figure out how to really relate [dsmap] to [dmap] *)
 
   Theorem dslookup_ok : forall lxp bxp ixp dnum name mscs,
-    {< F A mbase m flist f dsmap,
+    {< F A mbase m dsmap,
     PRE    MEMLOG.rep lxp (ActiveTxn mbase m) mscs *
-           rep f dsmap *
-           [[ (F * BFILE.rep bxp ixp flist)%pred (list2mem m) ]] *
-           [[ (A * dnum |-> f)%pred (list2mem flist) ]]
+           rep F A m bxp ixp dnum dsmap
     POST:(mscs',r)
            MEMLOG.rep lxp (ActiveTxn mbase m) mscs' *
            ((exists inum DF, [[ r = Some inum ]] *
